

# MAT215: Complex Variables And Laplace Transformations

Emon Hossain<sup>1</sup>

<sup>1</sup>Lecturer  
MNS department  
Brac University

LECTURE-05

# Derivative formula

## Example

Show that,

$$\mathcal{L}\{y'(t)\} = sY(s) - y(0)$$

## Example

Show that,

$$\mathcal{L}\{y''(t)\} = s^2Y(s) - sy(0) - y'(0)$$

## Example

Show that,

$$\mathcal{L}\{y'''(t)\} = s^3Y(s) - s^2y(0) - sy'(0) - y''(0)$$

# Example

## Example

Solve the given differential equation:

$$y'' - 4y' + 4y = t^3 e^{2t}, y(0) = 0, y'(0) = 0$$

## Example

Solve the given differential equation:

$$y'' - 3y' + 2y = 4, y(0) = 1, y'(0) = -1$$

**Hint:**

$$\frac{s-2}{s(s-1)} = \frac{2}{s} + \frac{-1}{s-1}$$

## Example

### Example

Solve the given differential equation:

$$y''' - 3y'' + 3y' - y = e^t t^2, y(0) = 0, y'(0) = 1, y''(0) = -2$$

### Example

Solve the given differential equation:

$$\frac{dy}{dt} + y = 13\sin 2t, y(0) = 6$$

**Hint:**

$$\frac{6s^2 + 50}{(s+3)(s^2+4)} = \frac{8}{(s+3)} + \frac{-2s+6}{(s^2+4)}$$

# Example

## Example

Solve the given differential equation:

$$2y''' + 3y'' - 3y' - 2y = e^{-t}, y(0) = 0, y'(0) = 0, y''(0) = 1$$

## Example

Solve the given differential equation:

$$y'' + 2y' + 5y = e^{-t} \sin t, y(0) = 0, y'(0) = 1$$

# Example

## Example

Solve the given differential equation:

$$y' + y = f(t), y(0) = 5$$

$$f(t) = \begin{cases} 0, & 0 \leq t < \pi \\ 2 \cos t, & t \geq \pi \end{cases}$$

## Example

Solve the given differential equation:

$$y'' + 4y = \sin tu(t - 2\pi), y(0) = 1, y'(0) = 0$$

## Example

Solve the given differential equation:

$$y'' + 9y = \cos 2t, y(0) = 0, y\left(\frac{\pi}{2}\right) = -1$$

## Example

Solve the given system of differential equations:

$$\frac{dx}{dt} = -x + y$$

$$\frac{dy}{dt} = 2x$$

with initial conditions  $x(0) = 0, y(0) = 1$ .

**Answer:**

$$x' = -x + y$$

$$sX(s) - x(0) = -X(s) + Y(s)$$

$$Y(s) = (s+1)X(s)$$



And,

$$y' = 2x$$

$$sY(s) - y(0) = 2X(s)$$

$$sY(s) - 1 = 2X(s)$$

$$2X(s) - s(s+1)X(s) = -1$$

$$X(s) = \frac{1}{s^2 + s - 2} = \frac{1/3}{s-1} + \frac{-1/3}{s+2}$$

$$x(t) = \frac{1}{3}e^t - \frac{1}{3}e^{-2t}$$

Now,

$$Y(s) = (s+1)X(s) = \frac{s+1}{s^2 + s - 2} = \frac{2/3}{s-1} + \frac{1/3}{s+2}$$

$$y(t) = \frac{2}{3}e^t + \frac{1}{3}e^{-2t}$$